matchesb_ext

minuska/theories/naive_interpreter.v
@@ -44,12 +44,70 @@ else
     None
 .
 
+Lemma merge_valuations_correct
+    {Σ : Signature}
+    (ρ1 ρ2 ρ : Valuation):
+    merge_valuations ρ1 ρ2 = Some ρ ->
+    ρ1 ⊆ ρ /\
+    ρ2 ⊆ ρ
+.
+Proof.
+    unfold Valuation in *.
+    unfold merge_valuations.
+    unfold is_left.
+    destruct (decide (valuations_compatible ρ1 ρ2)) as [Hcompat|Hnocompat]; intros H.
+    {
+        inversion H; subst; clear H.
+        unfold valuations_compatible in Hcompat.
+        unfold is_true in Hcompat.
+        rewrite forallb_forall in Hcompat; cbn.
+        ltac1:(setoid_rewrite <- elem_of_list_In in Hcompat).
+        ltac1:(setoid_rewrite elem_of_elements in Hcompat).
+        split; intros i;
+            destruct (ρ1 !! i) eqn:Hρ1i;
+            destruct (ρ2 !! i) eqn:Hρ2i;
+            destruct (merge use_left ρ1 ρ2 !! i) eqn:Hmergei;
+            simpl;
+            try (exact I);
+            ltac1:(rewrite lookup_merge in Hmergei);
+            unfold diag_None in Hmergei;
+            specialize (Hcompat i);
+            ltac1:(rewrite Hρ1i in Hmergei);
+            ltac1:(rewrite Hρ2i in Hmergei);
+            unfold use_left in Hmergei;
+            ltac1:(simplify_eq /=);
+            try reflexivity
+        .
+        
+        ltac1:(ospecialize (Hcompat _)).
+        {
+            rewrite elem_of_intersection.
+            do 2 ltac1:(rewrite elem_of_dom).
+            split; eexists.
+            {
+                apply Hρ1i.
+            }
+            {
+                apply Hρ2i.
+            }
+        }
+        apply bool_decide_eq_true_1 in Hcompat.
+        unfold Valuation in *.
+        rewrite Hcompat in Hρ1i.
+        rewrite Hρ1i in Hρ2i.
+        ltac1:(congruence).
+    }
+    {
+        inversion H.
+    }
+Qed.
+
 Class TryMatch
     {Σ : Signature}
     (A B : Type)
     {_VB: VarsOf B}
-    {_SAB : Satisfies (Valuation*A) B}
-    {_MAB : Matches (Valuation*A) B}
+    {_SAB : Satisfies Valuation A B}
+    {_MAB : Matches Valuation A B}
     :=
 {
     try_match :
@@ -58,11 +116,11 @@ Class TryMatch
     try_match_correct :
         ∀ (a : A) (b : B) (ρ : Valuation),
             try_match a b = Some ρ ->
-            matchesb (ρ,a) b = true ;
+            matchesb ρ a b = true ;
 
     try_match_complete :
         ∀ (a : A) (b : B) (ρ : Valuation),
-            matchesb (ρ,a) b = true ->
+            matchesb ρ a b = true ->
             ∃ (ρ' : Valuation),
                 vars_of ρ' = vars_of b /\
                 map_subseteq ρ' ρ /\
@@ -73,14 +131,14 @@ Fixpoint ApppliedOperator'_try_match_AppliedOperator'
     {Σ : Signature}
     {Operand1 Operand2 : Type}
     {_VOperand2 : VarsOf Operand2}
-    {_S0 : Satisfies (Valuation*Operand1) Operand2}
-    {_M0 : Matches (Valuation*Operand1) Operand2}
+    {_S0 : Satisfies Valuation (Operand1) Operand2}
+    {_M0 : Matches Valuation (Operand1) Operand2}
     {_TM0 : TryMatch Operand1 Operand2}
-    {_S1 : Satisfies (Valuation*Operand1) (AppliedOperator' symbol Operand2)}
-    {_M1 : Matches (Valuation*Operand1) (AppliedOperator' symbol Operand2)}
+    {_S1 : Satisfies Valuation (Operand1) (AppliedOperator' symbol Operand2)}
+    {_M1 : Matches Valuation (Operand1) (AppliedOperator' symbol Operand2)}
     {_TM1 : TryMatch Operand1 (AppliedOperator' symbol Operand2)}
-    {_TM2 : Satisfies (Valuation*(AppliedOperator' symbol Operand1)) Operand2}
-    {_TM2 : Matches (Valuation*(AppliedOperator' symbol Operand1)) Operand2}
+    {_TM2 : Satisfies Valuation ((AppliedOperator' symbol Operand1)) Operand2}
+    {_TM2 : Matches Valuation ((AppliedOperator' symbol Operand1)) Operand2}
     {_TM2 : TryMatch (AppliedOperator' symbol Operand1) Operand2}
     (x : AppliedOperator' symbol Operand1)
     (y : AppliedOperator' symbol Operand2)
@@ -131,223 +189,131 @@ Lemma ApppliedOperatorOr'_try_match_AppliedOperatorOr'_correct
     {Σ : Signature}
     {Operand1 Operand2 : Type}
     {_VOperand2 : VarsOf Operand2}
-    {_S0 : Satisfies (Valuation*Operand1) Operand2}
-    {_M0 : Matches (Valuation*Operand1) Operand2}
+    {_S0 : Satisfies Valuation (Operand1) Operand2}
+    {_M0 : Matches Valuation (Operand1) Operand2}
     {_TM0 : TryMatch Operand1 Operand2}
-    {_S1 : Satisfies (Valuation*Operand1) (AppliedOperator' symbol Operand2)}
-    {_M1 : Matches (Valuation*Operand1) (AppliedOperator' symbol Operand2)}
+    {_S1 : Satisfies Valuation (Operand1) (AppliedOperator' symbol Operand2)}
+    {_M1 : Matches Valuation (Operand1) (AppliedOperator' symbol Operand2)}
     {_TM1 : TryMatch Operand1 (AppliedOperator' symbol Operand2)}
-    {_TM2 : Satisfies (Valuation*(AppliedOperator' symbol Operand1)) Operand2}
-    {_TM2 : Matches (Valuation*(AppliedOperator' symbol Operand1)) Operand2}
+    {_S2 : Satisfies Valuation ((AppliedOperator' symbol Operand1)) Operand2}
+    {_M2 : Matches Valuation ((AppliedOperator' symbol Operand1)) Operand2}
     {_TM2 : TryMatch (AppliedOperator' symbol Operand1) Operand2}
-        (ρ ρ' : Valuation)
-        (a : AppliedOperator' symbol builtin_value)
-        (b : AppliedOperator' symbol BuiltinOrVar)
-        :
-        map_subseteq ρ ρ' ->
-        @ApppliedOperator'_try_match_AppliedOperator'
-            symbol _ builtin_value BuiltinOrVar
-            builtin_value_try_match_BuiltinOrVar
-            (fun _ _ => None)
-            pure_GroundTerm_try_match_BuiltinOrVar
-            a b = Some ρ ->
-
-        @ApppliedOperator'_matches_AppliedOperator'
-            symbol _ builtin_value BuiltinOrVar
-            builtin_value_matches_BuiltinOrVar
-            (fun _ _ _ => false)
-            pure_GroundTerm_matches_BuiltinOrVar
-            ρ' a b = true
-    .
-    Proof.
-        revert b ρ ρ'.
-        induction a; intros b' ρ ρ' HH H; destruct b'; cbn in *; intros.
+    (ρ ρ' : Valuation)
+    (a : AppliedOperator' symbol Operand1)
+    (b : AppliedOperator' symbol Operand2)
+    :
+    ρ ⊆ ρ' ->
+    ApppliedOperator'_try_match_AppliedOperator' a b = Some ρ ->
+    matchesb ρ' a b = true
+.
+Proof.
+    revert b ρ ρ'.
+    induction a; intros b' ρ ρ' HH H; destruct b'; cbn in *; intros.
+    {
+        intros.
+        unfold is_left in *.
+        unfold decide,bool_decide in *.
+        repeat ltac1:(case_match); subst; simpl;
+            try reflexivity; try ltac1:(congruence).
         {
-            intros.
-            unfold is_left in *.
-            unfold bool_decide.
-            repeat ltac1:(case_match); subst; simpl;
-                try reflexivity; ltac1:(congruence).
-        }
-        {
-            inversion H.
-        }
-        {
-            inversion H.
-        }
-        {
-            inversion H.
-        }
-        {
-            rewrite bind_Some in H.
-            destruct H as [x [H21 H22]].
-            rewrite bind_Some in H22.
-            destruct H22 as [x0 [H221 H222]].
-
-            assert (H221' := H221).
-            apply builtin_value_try_match_BuiltinOrVar_correct in H221.
-            assert (H222' := H222).
-            apply merge_valuations_correct in H222'.
-            destruct H222' as [Hsub1 Hsub2].
-            destruct H221 as [H2211 H2212].
-            cbn.
-            destruct H2212 as [HH1|HH2].
-            {
-                subst.
-                cbn.
-                unfold bool_decide.
-                repeat ltac1:(case_match).
-                rewrite andb_true_r.
-                (*
-                eapply matches_monotone.
-                { apply HH. }
-                *)
-                clear e H.
-                cbn in *.
-                clear H2211.
-                destruct (decide (b = b))>[|ltac1:(congruence)].
-                cbn in *.
-                inversion H221'; subst; clear H221'.
-                clear e.
-                rewrite merge_valuations_empty_r in H222.
-                inversion H222; subst; clear H222.
-                clear Hsub2.
-                clear Hsub1.
-                specialize (IHa b' ρ ρ' HH).
-                apply IHa.
-                apply H21.
+            ltac1:(simplify_eq/=).
+            unfold matchesb. simpl.
+            unfold bool_decide; ltac1:(case_match); subst;
                 ltac1:(congruence).
-            }
-            {
-                destruct HH2 as [x1 [HH3 HH4]].
-                subst.
-                cbn in *.
-                inversion H221'; subst; clear H221'.
-                ltac1:(rewrite lookup_insert in H2211).
-                clear H2211.
-                assert (Htmp: ρ' !! x1 = Some (aoo_operand symbol builtin_value b)).
-                {
-                    clear -Hsub2 HH.
-                    unfold map_subseteq in *.
-                    unfold map_included in *.
-                    unfold map_relation in *.
-                    unfold option_relation in *.
-                    specialize (HH x1).
-                    specialize (Hsub2 x1).
-                    repeat ltac1:(case_match); subst;
-                        ltac1:(rewrite lookup_insert in H);
-                        inversion H; subst; clear H;
-                        try assumption;
-                        try ltac1:(contradiction).
-                }
-                unfold Valuation_lookup in *.
-                rewrite Htmp.
-                unfold bool_decide.
-                ltac1:(case_match); try reflexivity; try ltac1:(congruence).
-                clear e H.
-                clear HH4.
-                assert (Htmp2 := IHa b').
-                remember (ApppliedOperator'_matches_AppliedOperator' symbol builtin_value
-                    BuiltinOrVar builtin_value_matches_BuiltinOrVar
-                    (λ (_ : Valuation) (_ : builtin_value) (_ : AppliedOperator'
-                    symbol
-                    BuiltinOrVar),
-                    false)
-                    pure_GroundTerm_matches_BuiltinOrVar)
-                as f.
-                remember (ApppliedOperator'_try_match_AppliedOperator' symbol
-                    builtin_value BuiltinOrVar
-                    builtin_value_try_match_BuiltinOrVar
-                    (λ (_ : builtin_value) (_ : AppliedOperator' symbol
-                    BuiltinOrVar),
-                    None)
-                    pure_GroundTerm_try_match_BuiltinOrVar)
-                as g.
-                apply Htmp2 with (ρ' := ρ') in H21.
-                {
-                    rewrite H21. reflexivity.
-                }
-                {
-                    eapply transitivity.
-                    { apply Hsub1. }
-                    { apply HH. }
-                }
-            }
+        }
+    }
+    {
+        inversion H.
+    }
+    {
+        inversion H.
+    }
+    {
+        inversion H.
+    }
+    {
+        rewrite bind_Some in H.
+        destruct H as [x [H21 H22]].
+        rewrite bind_Some in H22.
+        destruct H22 as [x0 [H221 H222]].
+        
+
+        assert (H221' := H221).
+        apply try_match_correct in H221.
+        assert (H222' := H222).
+        apply merge_valuations_correct in H222'.
+        destruct H222' as [Hsub1 Hsub2].
+
+        assert (IH := IHa _ _ _ Hsub1 H21).
+        unfold matchesb; simpl.
+        unfold matchesb in IH; simpl in IH.
+        rewrite IH; simpl.
+
+        destruct H221 as [H2211 H2212].
+        cbn.
+        destruct H2212 as [HH1|HH2].
+        {
+            subst.
+            cbn.
+            unfold bool_decide.
+            repeat ltac1:(case_match).
+            rewrite andb_true_r.
+            (*
+            eapply matches_monotone.
+            { apply HH. }
+            *)
+            clear e H.
+            cbn in *.
+            clear H2211.
+            destruct (decide (b = b))>[|ltac1:(congruence)].
+            cbn in *.
+            inversion H221'; subst; clear H221'.
+            clear e.
+            rewrite merge_valuations_empty_r in H222.
+            inversion H222; subst; clear H222.
+            clear Hsub2.
+            clear Hsub1.
+            specialize (IHa b' ρ ρ' HH).
+            apply IHa.
+            apply H21.
+            ltac1:(congruence).
         }
         {
-            rewrite bind_Some in H.
-            destruct H as [x [H21 H22]].
-            inversion H22.
-        }
-        {
-            inversion H.
-        }
-        {
-            rewrite bind_Some in H.
-            destruct H as [x [H21 H22]].
-            rewrite bind_Some in H22.
-            destruct H22 as [x0 [H221 H222]].
-            (* TODO: need a lemma about correctness of pure_GroundTerm_try_match_BuiltinOrVar *)
-            apply pure_GroundTerm_try_match_BuiltinOrVar_correct in H221.
-            assert (Hmv := H222).
-            apply merge_valuations_correct in Hmv.
-            destruct Hmv as [Hsub1 Hsub2].
-            assert (Hxrho': map_subseteq x ρ').
+            destruct HH2 as [x1 [HH3 HH4]].
+            subst.
+            cbn in *.
+            inversion H221'; subst; clear H221'.
+            ltac1:(rewrite lookup_insert in H2211).
+            clear H2211.
+            assert (Htmp: ρ' !! x1 = Some (aoo_operand symbol builtin_value b)).
             {
-                eapply transitivity.
-                apply Hsub1.
-                apply HH.
+                clear -Hsub2 HH.
+                unfold map_subseteq in *.
+                unfold map_included in *.
+                unfold map_relation in *.
+                unfold option_relation in *.
+                specialize (HH x1).
+                specialize (Hsub2 x1).
+                repeat ltac1:(case_match); subst;
+                    ltac1:(rewrite lookup_insert in H);
+                    inversion H; subst; clear H;
+                    try assumption;
+                    try ltac1:(contradiction).
             }
-            apply pure_GroundTerm_matches_BuiltinOrVar_monotone with (ρ' := ρ') in H221.
-            {
-                rewrite H221.
-                clear H221.
-                remember (ApppliedOperator'_try_match_AppliedOperator' symbol
-                    builtin_value BuiltinOrVar
-                    builtin_value_try_match_BuiltinOrVar
-                    (λ (_ : builtin_value) (_ : AppliedOperator' symbol
-                    BuiltinOrVar),
-                    None)
-                    pure_GroundTerm_try_match_BuiltinOrVar)
-                as f.
-                specialize (IHa1 b' x ρ' Hxrho' H21).
-                rewrite IHa1.
-                reflexivity.
-            }
-            {
-                eapply transitivity.
-                apply Hsub2.
-                apply HH.
-            }
-        }
-        {
-            rewrite bind_Some in H.
-            destruct H as [x [H21 H22]].
-            rewrite bind_Some in H22.
-            destruct H22 as [x0 [H221 H222]].
-            assert (Hsub := H222).
-            apply merge_valuations_correct in Hsub.
-            destruct Hsub as [Hsub1 Hsub2].
-            assert (Hxρ' : map_subseteq x ρ').
-            {
-                eapply transitivity.
-                apply Hsub1.
-                apply HH.
-            }
-            assert (Hx0ρ' : map_subseteq x0 ρ').
-            {
-                eapply transitivity.
-                apply Hsub2.
-                apply HH.
-            }
-            remember (
-                ApppliedOperator'_matches_AppliedOperator' symbol builtin_value
+            unfold Valuation_lookup in *.
+            rewrite Htmp.
+            unfold bool_decide.
+            ltac1:(case_match); try reflexivity; try ltac1:(congruence).
+            clear e H.
+            clear HH4.
+            assert (Htmp2 := IHa b').
+            remember (ApppliedOperator'_matches_AppliedOperator' symbol builtin_value
                 BuiltinOrVar builtin_value_matches_BuiltinOrVar
                 (λ (_ : Valuation) (_ : builtin_value) (_ : AppliedOperator'
                 symbol
                 BuiltinOrVar),
                 false)
-                pure_GroundTerm_matches_BuiltinOrVar )
+                pure_GroundTerm_matches_BuiltinOrVar)
             as f.
             remember (ApppliedOperator'_try_match_AppliedOperator' symbol
                 builtin_value BuiltinOrVar
@@ -357,12 +323,106 @@ Lemma ApppliedOperatorOr'_try_match_AppliedOperatorOr'_correct
                 None)
                 pure_GroundTerm_try_match_BuiltinOrVar)
             as g.
-            apply andb_true_iff.
-            ltac1:(naive_solver).
+            apply Htmp2 with (ρ' := ρ') in H21.
+            {
+                rewrite H21. reflexivity.
+            }
+            {
+                eapply transitivity.
+                { apply Hsub1. }
+                { apply HH. }
+            }
         }
-        Unshelve.
-        all: apply map_subseteq_po.
-    Qed.
+    }
+    {
+        rewrite bind_Some in H.
+        destruct H as [x [H21 H22]].
+        inversion H22.
+    }
+    {
+        inversion H.
+    }
+    {
+        rewrite bind_Some in H.
+        destruct H as [x [H21 H22]].
+        rewrite bind_Some in H22.
+        destruct H22 as [x0 [H221 H222]].
+        (* TODO: need a lemma about correctness of pure_GroundTerm_try_match_BuiltinOrVar *)
+        apply pure_GroundTerm_try_match_BuiltinOrVar_correct in H221.
+        assert (Hmv := H222).
+        apply merge_valuations_correct in Hmv.
+        destruct Hmv as [Hsub1 Hsub2].
+        assert (Hxrho': map_subseteq x ρ').
+        {
+            eapply transitivity.
+            apply Hsub1.
+            apply HH.
+        }
+        apply pure_GroundTerm_matches_BuiltinOrVar_monotone with (ρ' := ρ') in H221.
+        {
+            rewrite H221.
+            clear H221.
+            remember (ApppliedOperator'_try_match_AppliedOperator' symbol
+                builtin_value BuiltinOrVar
+                builtin_value_try_match_BuiltinOrVar
+                (λ (_ : builtin_value) (_ : AppliedOperator' symbol
+                BuiltinOrVar),
+                None)
+                pure_GroundTerm_try_match_BuiltinOrVar)
+            as f.
+            specialize (IHa1 b' x ρ' Hxrho' H21).
+            rewrite IHa1.
+            reflexivity.
+        }
+        {
+            eapply transitivity.
+            apply Hsub2.
+            apply HH.
+        }
+    }
+    {
+        rewrite bind_Some in H.
+        destruct H as [x [H21 H22]].
+        rewrite bind_Some in H22.
+        destruct H22 as [x0 [H221 H222]].
+        assert (Hsub := H222).
+        apply merge_valuations_correct in Hsub.
+        destruct Hsub as [Hsub1 Hsub2].
+        assert (Hxρ' : map_subseteq x ρ').
+        {
+            eapply transitivity.
+            apply Hsub1.
+            apply HH.
+        }
+        assert (Hx0ρ' : map_subseteq x0 ρ').
+        {
+            eapply transitivity.
+            apply Hsub2.
+            apply HH.
+        }
+        remember (
+            ApppliedOperator'_matches_AppliedOperator' symbol builtin_value
+            BuiltinOrVar builtin_value_matches_BuiltinOrVar
+            (λ (_ : Valuation) (_ : builtin_value) (_ : AppliedOperator'
+            symbol
+            BuiltinOrVar),
+            false)
+            pure_GroundTerm_matches_BuiltinOrVar )
+        as f.
+        remember (ApppliedOperator'_try_match_AppliedOperator' symbol
+            builtin_value BuiltinOrVar
+            builtin_value_try_match_BuiltinOrVar
+            (λ (_ : builtin_value) (_ : AppliedOperator' symbol
+            BuiltinOrVar),
+            None)
+            pure_GroundTerm_try_match_BuiltinOrVar)
+        as g.
+        apply andb_true_iff.
+        ltac1:(naive_solver).
+    }
+    Unshelve.
+    all: apply map_subseteq_po.
+Qed.
 
     Definition ApppliedOperatorOr'_try_match_AppliedOperatorOr'
         (Operator : Type)
@@ -833,60 +893,7 @@ Lemma ApppliedOperatorOr'_try_match_AppliedOperatorOr'_correct
         apply gmap_lookup.
     Defined.
     
-    Lemma merge_valuations_correct (ρ1 ρ2 ρ : Valuation):
-        merge_valuations ρ1 ρ2 = Some ρ ->
-        map_subseteq ρ1 ρ /\
-        map_subseteq ρ2 ρ
-    .
-    Proof.
-        unfold merge_valuations.
-        unfold is_left.
-        destruct (decide (valuations_compatible ρ1 ρ2)) as [Hcompat|Hnocompat]; intros H.
-        {
-            inversion H; subst; clear H.
-            unfold valuations_compatible in Hcompat.
-            rewrite Forall_forall in Hcompat; cbn.
-            ltac1:(setoid_rewrite <- elem_of_list_In in Hcompat).
-            ltac1:(setoid_rewrite elem_of_elements in Hcompat).
-            unfold map_subseteq.
-            unfold map_included.
-            unfold map_relation.
-            unfold option_relation.
-            fold (@Valuation Σ) in *.
-            fold (@Valuation_lookup) in *.
-            split; intros i;
-                destruct (ρ1 !! i) eqn:Hρ1i;
-                destruct (ρ2 !! i) eqn:Hρ2i;
-                destruct (merge use_left ρ1 ρ2 !! i) eqn:Hmergei;
-                ltac1:(rewrite Hmergei);
-                try (exact I);
-                ltac1:(rewrite lookup_merge in Hmergei);
-                unfold diag_None in Hmergei;
-                specialize (Hcompat i);
-                ltac1:(rewrite Hρ1i in Hmergei);
-                ltac1:(rewrite Hρ2i in Hmergei);
-                unfold use_left in Hmergei;
-                ltac1:(simplify_eq /=);
-                try reflexivity
-            .
-            ltac1:(ospecialize (Hcompat _)).
-            {
-                rewrite elem_of_intersection.
-                do 2 ltac1:(rewrite elem_of_dom).
-                split; eexists.
-                {
-                    apply Hρ1i.
-                }
-                {
-                    apply Hρ2i.
-                }
-            }
-            ltac1:(congruence).
-        }
-        {
-            inversion H.
-        }
-    Qed.
+    
 
     Lemma builtin_value_matches_BuiltinOrVar_monotone
         (ρ ρ' : Valuation)
